File reorganisation: states have a file of their own, now.

low/Monads.v
@@ -1,222 +1,11 @@
 (** Monads.
- * Provides some model for the C memory and some monads to manipulate it easily. **)
+ * Provides monads to manipulate R objects easily. **)
 
 Set Implicit Arguments.
-Require Export String.
-Require Export RinternalsAux TLC.LibHeap Shared.
-Require Import TLC.LibStream.
-
-(** * A Model for the C Memory **)
-
-(** ** Basic Model **)
-
-(** The global state of the C environment. In particular, it maps SEXP
- * pointers to their corresponding expressions. **)
-Record state := make_state {
-    state_heap_SExp :> heap nat SExpRec ;
-    state_fresh_locations : stream nat ;
-    state_fresh_locations_fresh : forall n,
-      ~ indom state_heap_SExp (LibStream.nth n state_fresh_locations) ;
-    state_fresh_locations_different : forall n1 n2,
-      n1 <> n2 ->
-      LibStream.nth n1 state_fresh_locations <> LibStream.nth n2 state_fresh_locations
-  }.
-
-(** Allocate a new cell and provide it an initial value **)
-Definition alloc_SExp_nat (S : state) (e : SExpRec) : state * nat.
-  refine (let p := stream_head (state_fresh_locations S) in ({|
-      state_heap_SExp := write S p e ;
-      state_fresh_locations := stream_tail (state_fresh_locations S) |},
-    p)).
-  - introv I. rewrite stream_tail_nth in I. forwards~ I': @indom_write_inv I.
-    + unfolds p. rewrite stream_head_nth. applys* state_fresh_locations_different.
-    + applys~ state_fresh_locations_fresh I'.
-  - introv D. repeat rewrite stream_tail_nth. applys* state_fresh_locations_different.
-Defined.
-
-Definition alloc_SExp S e : state * SExpRec_pointer :=
-  let (S, p) := alloc_SExp_nat S e in
-  (S, Some p).
-
-(** Writes a value in the state. Might return [None] if the cell is not already allocated. **)
-Definition write_SExp_nat (S : state) (p : nat) (e : SExpRec) : option state.
-  refine (match read_option S p as r return r = _ -> _ with
-          | None => fun _ => None
-          | Some _ => fun Eq => Some {|
-              state_heap_SExp := write S p e ;
-              state_fresh_locations := state_fresh_locations S |}
-          end eq_refl).
-  - introv. apply not_indom_write.
-    + introv E. applys state_fresh_locations_fresh. rewrite E.
-      symmetry in Eq. applys~ read_option_indom Eq.
-    + applys~ state_fresh_locations_fresh.
-  - apply* state_fresh_locations_different.
-Defined.
-
-Definition write_SExp (S : state) (p : SExpRec_pointer) (e : SExpRec) :=
-  match p with
-  | None => None
-  | Some p => write_SExp_nat S p e
-  end.
-
-Definition read_SExp_nat (S : state) (p : nat) : option SExpRec :=
-  read_option S p.
-
-(** Reads a value in the state. **)
-Definition read_SExp (S : state) (p : SExpRec_pointer) :=
-  match p with
-  | None => None
-  | Some p => read_SExp_nat S p
-  end.
-
-Lemma alloc_SExp_nat_read_SExp : forall S S' e p,
-  alloc_SExp_nat S e = (S', p) ->
-  read_SExp S' (Some p) = Some e.
-Proof. introv Eq. inverts Eq. do 2 unfolds. simpl. rewrite~ read_option_write_same. Qed.
-
-Lemma alloc_SExp_read_SExp : forall S S' e p,
-  alloc_SExp S e = (S', p) ->
-  read_SExp S' p = Some e.
-Proof. introv Eq. inverts Eq. applys* alloc_SExp_nat_read_SExp. Qed.
-
-Lemma destruct_write_SExp_nat_None : forall (S : state) p e,
-  read_option S p = None ->
-  write_SExp_nat S p e = None.
-Proof.
-  introv E. unfolds.
-  asserts R: (forall T P (x : option T) (f1 : None = x -> P None) (f2 : forall v, Some v = x -> _)
-      (H : None = x),
-    match x as r return r = x -> P r with
-    | None => f1
-    | Some v => fun E => f2 v E
-    end eq_refl
-    = match H in _ = r return P r with
-      | eq_refl => f1 H
-      end).
-  + clear. introv. destruct~ H.
-  + symmetry in E. lets R': (rm R) (read_option S p). erewrite (R' _ _ E). destruct~ E.
-Qed.
-
-Lemma destruct_write_SExp_nat : forall (S : state) p e v,
-  read_option S p = Some v ->
-  exists S',
-    write_SExp_nat S p e = Some S'
-    /\ (S' : heap _ _) = write S p e.
-Proof.
-  introv E. unfolds write_SExp_nat.
-  asserts R: (forall T T' (x : option T) (f1 : None = x -> T') (f2 : forall v, Some v = x -> T')
-      v (H : Some v = x),
-    match x as r return r = x -> T' with
-    | None => f1
-    | Some v => fun E => f2 v E
-    end eq_refl
-    = f2 v H).
-  + clear. introv. destruct~ H.
-  + symmetry in E. lets R': (rm R) (read_option S p). rewrite (R' _ _ _ E). clear.
-    eexists. splits~.
-Qed.
-
-Lemma write_SExp_nat_read_SExp_same : forall S S' e p,
-  write_SExp_nat S p e = Some S' ->
-  read_SExp S' (Some p) = Some e.
-Proof.
-  introv E. simpl. destruct (read_option S p) eqn: E'.
-  + forwards (S2&E1&E2): destruct_write_SExp_nat E'.
-    rewrite E in E1. inverts E1. unfolds. rewrite E2. rewrite~ read_option_write_same.
-  + forwards Eq: destruct_write_SExp_nat_None E'. rewrite Eq in E. false*.
-Qed.
-
-Lemma write_SExp_read_SExp_same : forall S S' e p,
-  write_SExp S p e = Some S' ->
-  read_SExp S' p = Some e.
-Proof. introv E. destruct p; tryfalse. applys~ write_SExp_nat_read_SExp_same E. Qed.
-
-Lemma write_SExp_nat_read_SExp : forall S S' e p p',
-  write_SExp_nat S p e = Some S' ->
-  p <> p' ->
-  read_SExp S' (Some p') = read_SExp S (Some p').
-Proof.
-  introv E D. simpl. destruct (read_option S p) eqn: E'.
-  + forwards (S2&E1&E2): destruct_write_SExp_nat E'.
-    rewrite E in E1. inverts E1. unfolds. rewrite E2. rewrite~ read_option_write.
-  + forwards Eq: destruct_write_SExp_nat_None E'. rewrite Eq in E. false*.
-Qed.
-
-Lemma write_SExp_read_SExp : forall S S' e p p',
-  write_SExp S p e = Some S' ->
-  p <> p' ->
-  read_SExp S' p' = read_SExp S p'.
-Proof.
-  introv E D. destruct p; tryfalse. destruct p'.
-  + applys~ write_SExp_nat_read_SExp E.
-  + reflexivity.
-Qed.
-
-Lemma read_SExp_write_SExp_nat : forall S e e' p,
-  read_SExp S (Some p) = Some e ->
-  exists S', write_SExp_nat S p e' = Some S'.
-Proof.
-  introv E. simpl in E. forwards (S'&E1&E2): destruct_write_SExp_nat E.
-  exists S'. rewrite~ E1.
-Qed.
-
-Lemma read_SExp_write_SExp : forall S e e' p,
-  read_SExp S p = Some e ->
-  exists S', write_SExp S p e' = Some S'.
-Proof. introv E. destruct p; tryfalse. applys~ read_SExp_write_SExp_nat E. Qed.
+Require Export State.
 
 
-(* TODO: Do we need this? There is already allocList from Reval/memory.c
-(** ** Support for Arrays **)
-
-Fixpoint alloc_array_SExp S (es : list SExpRec) : state * SExpRec_pointer :=
-  match es with
-  | nil => (S, None)
-  | e :: es =>
-    let (S, p) := alloc_SExp S e in
-  end.
-
-Lemmae of the form: if the read is in the length of the array, then it succeeds.
-*)
-
-(** ** Initial Memory **)
-
-CoFixpoint all_locations n : stream nat :=
-  n ::: (all_locations (1 + n)).
-
-Lemma all_locations_nth : forall n m,
-  nth m (all_locations n) = m + n.
-Proof.
-  introv. gen n. induction m; introv.
-  - reflexivity.
-  - simpl. rewrite~ IHm.
-Qed.
-
-Definition empty_state : state.
-  refine {|
-      state_heap_SExp := empty ;
-      state_fresh_locations := all_locations 0
-    |}.
-  - introv. apply~ @not_indom_empty. typeclass.
-  - introv D. repeat rewrite all_locations_nth. math.
-Defined.
-
-
-(* TODO: Fix this. Also track “None” in the Coq and replace it by the corresponding value. *)
-Definition NULL : SExpRec_pointer := None.
-Definition R_NilValue : SExpRec_pointer := NULL. (* snd (alloc_SExp empty_state Nil_SExpRec). *)
-Definition R_DotsSymbol : SExpRec_pointer := NULL. (* TODO: See names.c *)
-Definition R_GlobalEnv : SExpRec_pointer := NULL. (* TODO: See envir.c *)
-Definition R_EmptyEnv : SExpRec_pointer := NULL. (* TODO: See envir.c *)
-Definition R_BaseEnv : SExpRec_pointer := NULL. (* TODO: See envir.c *)
-Definition R_UnboundValue : SExpRec_pointer := NULL. (* TODO: See names.c *)
-Definition R_MissingArg : SExpRec_pointer := NULL. (* TODO: See names.c *)
-Definition initial_state := empty_state. (*fst (alloc_SExp empty_state ?).*)
-
-
-(** * Monads **)
-
-(** ** Monadic Type **)
+(** * Monadic Type **)
 
 (** A monad type for results. **)
 Inductive result (A : Type) :=
@@ -250,7 +39,7 @@ Arguments result_bottom [A].
  * return [result_impossible]. **)
 
 
-(** ** Generic Monads **)
+(** * Generic Monads **)
 
 (** The monad for result. **)
 Definition if_success (A B : Type) (r : result A) (f : state -> A -> result B) : result B :=
@@ -301,7 +90,7 @@ Definition set_tag A S tag (p : SExpRec_pointer) (f : state -> result A) : resul
   map_list S (set_tag_list tag) p f.
 
 
-(** ** Monads to View Basic Language Elements Differently **)
+(** * Monads to View Basic Language Elements Differently **)
 
 Definition if_is_sym A S (e_ : SExpRec) (f : NonVector_SExpRec -> SymSxp_struct -> result A) : result A :=
   if_defined S (get_NonVector e_) (fun e_ =>
