low/State.v
@@ -1,0 +1,234 @@
+(** Monads.
+ * Provides a model for the C memory, as well as most R global variables. **)
+
+Set Implicit Arguments.
+Require Export String.
+Require Export RinternalsAux TLC.LibHeap Shared.
+Require Import TLC.LibStream.
+
+
+(** * A Model for the C Memory **)
+
+(** The global state of the C memory. In particular, it maps SEXP
+ * pointers to their corresponding expressions. **)
+Record memory := make_memory {
+    state_heap_SExp :> heap nat SExpRec ;
+    state_fresh_locations : stream nat ;
+    state_fresh_locations_fresh : forall n,
+      ~ indom state_heap_SExp (LibStream.nth n state_fresh_locations) ;
+    state_fresh_locations_different : forall n1 n2,
+      n1 <> n2 ->
+      LibStream.nth n1 state_fresh_locations <> LibStream.nth n2 state_fresh_locations
+  }.
+
+(** Allocate a new cell and provide it an initial value **)
+Definition alloc_memory_SExp_nat (S : memory) (e_ : SExpRec) : memory * nat.
+  refine (let p := stream_head (state_fresh_locations S) in ({|
+      state_heap_SExp := write S p e_ ;
+      state_fresh_locations := stream_tail (state_fresh_locations S) |},
+    p)).
+  - introv I. rewrite stream_tail_nth in I. forwards~ I': @indom_write_inv I.
+    + unfolds p. rewrite stream_head_nth. applys* state_fresh_locations_different.
+    + applys~ state_fresh_locations_fresh I'.
+  - introv D. repeat rewrite stream_tail_nth. applys* state_fresh_locations_different.
+Defined.
+
+Definition alloc_memory_SExp S e_ : memory * SExpRec_pointer :=
+  let (S, p) := alloc_memory_SExp_nat S e_ in
+  (S, Some p).
+
+(** Writes a value in the state. Might return [None] if the cell is not already allocated. **)
+Definition write_memory_SExp_nat (S : memory) (e : nat) (e_ : SExpRec) : option memory.
+  refine (match read_option S e as r return r = _ -> _ with
+          | None => fun _ => None
+          | Some _ => fun Eq => Some {|
+              state_heap_SExp := write S e e_ ;
+              state_fresh_locations := state_fresh_locations S |}
+          end eq_refl).
+  - introv. apply not_indom_write.
+    + introv E. applys state_fresh_locations_fresh. rewrite E.
+      symmetry in Eq. applys~ read_option_indom Eq.
+    + applys~ state_fresh_locations_fresh.
+  - apply* state_fresh_locations_different.
+Defined.
+
+Definition write_memory_SExp (S : memory) (e : SExpRec_pointer) (e_ : SExpRec) :=
+  match e with
+  | None => None
+  | Some e => write_memory_SExp_nat S e e_
+  end.
+
+Definition read_SExp_nat (S : memory) (e : nat) : option SExpRec :=
+  read_option S e.
+
+(** Reads a value in the state. **)
+Definition read_SExp (S : memory) (e : SExpRec_pointer) :=
+  match e with
+  | None => None
+  | Some e => read_SExp_nat S e
+  end.
+
+Lemma alloc_memory_SExp_nat_read_SExp : forall S S' e_ e,
+  alloc_memory_SExp_nat S e_ = (S', e) ->
+  read_SExp S' (Some e) = Some e_.
+Proof. introv Eq. inverts Eq. do 2 unfolds. simpl. rewrite~ read_option_write_same. Qed.
+
+Lemma alloc_memory_SExp_read_SExp : forall S S' e_ e,
+  alloc_memory_SExp S e_ = (S', e) ->
+  read_SExp S' e = Some e_.
+Proof. introv Eq. inverts Eq. applys* alloc_memory_SExp_nat_read_SExp. Qed.
+
+Lemma destruct_write_memory_SExp_nat_None : forall (S : memory) e e_,
+  read_option S e = None ->
+  write_memory_SExp_nat S e e_ = None.
+Proof.
+  introv E. unfolds.
+  asserts R: (forall T P (x : option T) (f1 : None = x -> P None) (f2 : forall v, Some v = x -> _)
+      (H : None = x),
+    match x as r return r = x -> P r with
+    | None => f1
+    | Some v => fun E => f2 v E
+    end eq_refl
+    = match H in _ = r return P r with
+      | eq_refl => f1 H
+      end).
+  + clear. introv. destruct~ H.
+  + symmetry in E. lets R': (rm R) (read_option S e). erewrite (R' _ _ E). destruct~ E.
+Qed.
+
+Lemma destruct_write_memory_SExp_nat : forall (S : memory) e e_ v,
+  read_option S e = Some v ->
+  exists S',
+    write_memory_SExp_nat S e e_ = Some S'
+    /\ (S' : heap _ _) = write S e e_.
+Proof.
+  introv E. unfolds write_memory_SExp_nat.
+  asserts R: (forall T T' (x : option T) (f1 : None = x -> T') (f2 : forall v, Some v = x -> T')
+      v (H : Some v = x),
+    match x as r return r = x -> T' with
+    | None => f1
+    | Some v => fun E => f2 v E
+    end eq_refl
+    = f2 v H).
+  + clear. introv. destruct~ H.
+  + symmetry in E. lets R': (rm R) (read_option S e). rewrite (R' _ _ _ E). clear.
+    eexists. splits~.
+Qed.
+
+Lemma write_memory_SExp_nat_read_SExp_same : forall S S' e_ e,
+  write_memory_SExp_nat S e e_ = Some S' ->
+  read_SExp S' (Some e) = Some e_.
+Proof.
+  introv E. simpl. destruct (read_option S e) eqn: E'.
+  + forwards (S2&E1&E2): destruct_write_memory_SExp_nat E'.
+    rewrite E in E1. inverts E1. unfolds. rewrite E2. rewrite~ read_option_write_same.
+  + forwards Eq: destruct_write_memory_SExp_nat_None E'. rewrite Eq in E. false*.
+Qed.
+
+Lemma write_memory_SExp_read_SExp_same : forall S S' e_ e,
+  write_memory_SExp S e e_ = Some S' ->
+  read_SExp S' e = Some e_.
+Proof. introv E. destruct e; tryfalse. applys~ write_memory_SExp_nat_read_SExp_same E. Qed.
+
+Lemma write_memory_SExp_nat_read_SExp : forall S S' e_ e e',
+  write_memory_SExp_nat S e e_ = Some S' ->
+  e <> e' ->
+  read_SExp S' (Some e') = read_SExp S (Some e').
+Proof.
+  introv E D. simpl. destruct (read_option S e) eqn: E'.
+  + forwards (S2&E1&E2): destruct_write_memory_SExp_nat E'.
+    rewrite E in E1. inverts E1. unfolds. rewrite E2. rewrite~ read_option_write.
+  + forwards Eq: destruct_write_memory_SExp_nat_None E'. rewrite Eq in E. false*.
+Qed.
+
+Lemma write_memory_SExp_read_SExp : forall S S' e_ e e',
+  write_memory_SExp S e e_ = Some S' ->
+  e <> e' ->
+  read_SExp S' e' = read_SExp S e'.
+Proof.
+  introv E D. destruct e; tryfalse. destruct e'.
+  + applys~ write_memory_SExp_nat_read_SExp E.
+  + reflexivity.
+Qed.
+
+Lemma read_SExp_write_memory_SExp_nat : forall S e_ e'_ e,
+  read_SExp S (Some e) = Some e_ ->
+  exists S', write_memory_SExp_nat S e e'_ = Some S'.
+Proof.
+  introv E. simpl in E. forwards (S'&E1&E2): destruct_write_memory_SExp_nat E.
+  exists S'. rewrite~ E1.
+Qed.
+
+Lemma read_SExp_write_memory_SExp : forall S e_ e'_ e,
+  read_SExp S e = Some e_ ->
+  exists S', write_memory_SExp S e e'_ = Some S'.
+Proof. introv E. destruct e; tryfalse. applys~ read_SExp_write_memory_SExp_nat E. Qed.
+
+
+(** * A Model for R’s State **)
+
+Record state := make_state {
+    state_memory :> memory
+  }.
+
+
+Definition state_with_memory (S : state) m := {|
+    state_memory := m
+  |}.
+
+Definition alloc_SExp (S : state) e_ :=
+  let (m, e) := alloc_memory_SExp S e_ in
+  (state_with_memory S m, e).
+
+Definition write_SExp (S : state) e e_ :=
+  match write_memory_SExp S e e_ with
+  | Some m => Some (state_with_memory S m)
+  | None => None
+  end.
+
+
+(** * Initial State **)
+
+(** ** Initial Memory **)
+
+CoFixpoint all_locations n : stream nat :=
+  n ::: (all_locations (1 + n)).
+
+Lemma all_locations_nth : forall n m,
+  nth m (all_locations n) = m + n.
+Proof.
+  introv. gen n. induction m; introv.
+  - reflexivity.
+  - simpl. rewrite~ IHm.
+Qed.
+
+Definition empty_memory : memory.
+  refine {|
+      state_heap_SExp := empty ;
+      state_fresh_locations := all_locations 0
+    |}.
+  - introv. apply~ @not_indom_empty. typeclass.
+  - introv D. repeat rewrite all_locations_nth. math.
+Defined.
+
+
+(* TODO: Fix this. Also track “None” in the Coq and replace it by the corresponding value. *)
+Definition NULL : SExpRec_pointer := None.
+Definition R_NilValue : SExpRec_pointer := NULL. (* snd (alloc_SExp empty_state Nil_SExpRec). *)
+Definition R_DotsSymbol : SExpRec_pointer := NULL. (* TODO: See names.c *)
+Definition R_GlobalEnv : SExpRec_pointer := NULL. (* TODO: See envir.c *)
+Definition R_EmptyEnv : SExpRec_pointer := NULL. (* TODO: See envir.c *)
+Definition R_BaseEnv : SExpRec_pointer := NULL. (* TODO: See envir.c *)
+Definition R_UnboundValue : SExpRec_pointer := NULL. (* TODO: See names.c *)
+Definition R_MissingArg : SExpRec_pointer := NULL. (* TODO: See names.c *)
+
+
+(** ** Initial State **)
+
+Definition empty_state := {|
+    state_memory := empty_memory
+  |}.
+
+Definition initial_state := empty_state.
+
+
